Big step - unfinished

Com.thy
@@ -1,13 +1,12 @@
 theory Com imports BExp
 begin
 
-datatype com = 
-    SKIP
-  | Assign vname aexp     ("_ ::= _" [1000, 61] 61)
-  | Seq    com com        ("_;;/ _"  [60, 61] 60)
-  | If     bexp com com   ("(IF _/ THEN _/ ELSE _)" [0, 0, 61] 61)
-  | While  bexp com       ("(WHILE _/ DO _)" [0, 61] 61)
-
+datatype
+  com = SKIP
+      | Assign vname aexp       ("_ ::= _" [1000, 61] 61)
+      | Seq    com  com         ("_;;/ _"  [60, 61] 60)
+      | If     bexp com com     ("(IF _/ THEN _/ ELSE _)"  [0, 0, 61] 61)
+      | While  bexp com         ("(WHILE _/ DO _)"  [0, 61] 61)
 
 value "''x'' ::= Plus (V ''y'') (N 1);; ''y'' ::= N 2"
 
