Big_Step.thy
@@ -28,4 +28,114 @@ values "{map t [''x''] |t. (SKIP, <''x'' := 42>) \<Rightarrow> t}"
 
 values "{map t[''x'', ''y''] |t. (''x'' ::= N 2, \<lambda>_. 0) \<Rightarrow> t}"
 
+declare big_step.intros [intro]
+
+thm big_step.induct
+
+lemmas big_step_induct = big_step.induct[split_format(complete)]
+thm big_step_induct
+
+inductive_cases SkipE[elim!]: "(SKIP,s) \<Rightarrow> t"
+thm SkipE
+
+inductive_cases AssignE[elim!]: "(x ::= a,s) \<Rightarrow> t"
+thm AssignE
+inductive_cases SeqE[elim!]: "(c1;;c2,s1) \<Rightarrow> s3"
+thm SeqE
+inductive_cases IfE[elim!]: "(IF b THEN c1 ELSE c2,s) \<Rightarrow> t"
+thm IfE
+
+inductive_cases WhileE[elim]: "(WHILE b DO c,s) \<Rightarrow> t"
+thm WhileE
+
+lemma "(IF b THEN SKIP ELSE SKIP, s) \<Rightarrow> t \<Longrightarrow> t = s"
+  by blast
+
+thm IfTrue
+
+lemma assumes "(IF b THEN SKIP ELSE SKIP, s) \<Rightarrow> t" shows "t = s"
+proof -
+  from assms show ?thesis
+  proof cases
+    case IfTrue thm IfTrue
+    thus ?thesis by blast
+  next
+    case IfFalse thus ?thesis by blast
+  qed
+qed
+
+(*
+for some reason auto didn't work for the lemma below
+
+lemma assign_simp: "(x ::= a,s) \<Rightarrow> s' \<longleftrightarrow> (s' = s(x := aval a s))"
+  by auto
+*)
+
+
+
+lemma Seq_assoc: "(c1;; c2;; c3, s) \<Rightarrow> s' \<longleftrightarrow> (c1;; (c2;; c3), s) \<Rightarrow> s'"
+proof
+  assume "(c1;; c2;; c3, s) \<Rightarrow> s'"
+  then obtain s1 s2 where
+  c1: "(c1, s) \<Rightarrow> s1" and
+  c2: "(c2, s1) \<Rightarrow> s2" and
+  c3: "(c3, s2) \<Rightarrow> s'" by auto
+  from c2 c3
+  have "(c2;; c3, s1) \<Rightarrow> s'" by (rule Seq)
+  with c1
+  show "(c1;; (c2;; c3), s) \<Rightarrow> s'" by (rule Seq)
+next
+  assume "(c1;; (c2;; c3), s) \<Rightarrow> s'"
+  thus "(c1;; c2;; c3, s) \<Rightarrow> s'" by auto
+qed
+
+abbreviation
+  equiv_c :: "com \<Rightarrow> com \<Rightarrow> bool" (infix "\<sim>" 50) where
+  "c \<sim> c' \<equiv> (\<forall> s t. (c,s) \<Rightarrow> t = (c',s) \<Rightarrow> t)"
+  
+lemma while_unfold:
+  "(WHILE b DO c) \<sim> (IF b THEN c;; WHILE b DO c ELSE SKIP)"
+  by blast
+
+lemma triv_if:
+  "(IF b THEN c ELSE c) \<sim> c"
+  by blast
+
+lemma commute_if:
+  "(IF b1 THEN (IF b2 THEN c11 ELSE c12) ELSE c2) 
+   \<sim> 
+   (IF b2 THEN (IF b1 THEN c11 ELSE c2) ELSE (IF b1 THEN c12 ELSE c2))"
+  by blast
+
+lemma sim_while_cong[simp]: "c \<sim> c' \<Longrightarrow> WHILE b DO c \<sim> WHILE b DO c'"
+  by blast
+
+lemma sim_while_cong_aux:
+  "(WHILE b DO c,s) \<Rightarrow> t  \<Longrightarrow> c \<sim> c' \<Longrightarrow>  (WHILE b DO c',s) \<Rightarrow> t"
+  by blast
+
+lemma sim_relf: "c \<sim> c" by simp
+lemma sim_sym: "(c \<sim> c') = (c' \<sim> c)" by auto
+lemma sim_trans: "c \<sim> c' \<Longrightarrow> c' \<sim> c'' \<Longrightarrow> c \<sim> c''" by auto
+
+(*
+theorem big_step_determ: "\<lbrakk> (c,s) \<Rightarrow> t; (c,s) \<Rightarrow> u \<rbrakk> \<Longrightarrow> u = t"
+  by (induction arbitrary: u rule: big_step.induct) blast+
+*)
+
+theorem "(c,s) \<Rightarrow> t  \<Longrightarrow>  (c,s) \<Rightarrow> t'  \<Longrightarrow>  t' = t"
+proof (induction arbitrary: t' rule: big_step.induct)
+  fix b c s s1 t t'
+  assume "bval b s" and "(c,s) \<Rightarrow> s1" and "(WHILE b DO c,s1) \<Rightarrow> t"
+  assume IHc: "\<And>t'. (c,s) \<Rightarrow> t' \<Longrightarrow> t' = s1"
+  assume IHw: "\<And>t'. (WHILE b DO c,s1) \<Rightarrow> t' \<Longrightarrow> t' = t"
+  assume "(WHILE b DO c,s) \<Rightarrow> t'"
+  with \<open>bval b s\<close> obtain s1' where
+      c: "(c,s) \<Rightarrow> s1'" and
+      w: "(WHILE b DO c,s1') \<Rightarrow> t'"
+    by auto
+  from c IHc have "s1' = s1" by blast
+  with w IHw show "t' = t" by blast
+qed blast+
+
 end
